lambek/LambekScript.sml
@@ -20,25 +20,20 @@
  *)
 
 (* Brief usage for non-HOL users: (Linux & Mac OS X only)
- * 1. Download & install Poly/ML 5.6 from http://www.polyml.org
- * 2. Download & install HOL4 (kananaskis-11) from https://hol-theorem-prover.org
- * 3. Put HOL4's "bin" directory into PATH;
- * 4. Execute `Holmake` in current directory (with LambekScript.sml)
- * 5. Check LambekTheory.sig for a list of all definitions and theorems
- * 6. Start HOL by executing `hol` in current directory
- * 7. Execute: load "LambekTheory";
- * 8. Execute: open LambekTheory;
+ *
+ *  1. Download & install Poly/ML 5.6 from http://www.polyml.org
+ *  2. Download & install HOL4 (kananaskis-11) from https://hol-theorem-prover.org
+ *  3. Put HOL4's "bin" directory into your PATH;
+ *  4. Execute `Holmake` in current directory (in qui si trova "LambekScript.sml")
+ *  5. Check LambekTheory.sig for a list of all definitions and theorems
+ *  6. Start HOL by executing `hol` in current directory
+ *  7. Execute: load "LambekTheory";
+ *  8. Execute: open LambekTheory;
  *)
 
-app load ["UnicodeChars"];
+open HolKernel Parse boolLib bossLib;
 
-open HolKernel Parse boolLib bossLib simpLib BasicProvers;
-
-(*
- val _ = HOL_Interactive.toggle_quietdec();
- *)
-
-open relationTheory;	(* RTC *)
+open relationTheory;
 
 val _ = new_theory "Lambek";
 
@@ -74,27 +69,6 @@ val extends_trans = store_thm ("extends_trans",
 val extends_transitive = store_thm ("extends_trans", ``transitive extends``,
     REWRITE_TAC [transitive_def, extends_trans]);
 
-(** most popular extensions **)
-
-val NL_def = Define `NL = EMPTY_REL`;
-
-val (L_rules, _ , _) = Hol_reln `
-    (!A B C. L (Dot A (Dot B C)) (Dot (Dot A B) C)) /\
-    (!A B C. L (Dot (Dot A B) C) (Dot A (Dot B C))) `;
-val (NLP_rules, _, _) = Hol_reln `
-    (!A B. NLP (Dot A B) (Dot B A)) `;
-
-val LP_def = Define `LP = add_extension NLP L`;
-
-val NL_X = store_thm ("NL_X", ``!X. extends NL X``,
-    RW_TAC std_ss [extends_def, NL_def, EMPTY_REL_DEF, RSUBSET]);
-
-val NLP_LP = store_thm ("NLP_LP", ``extends NLP LP``,
-    REWRITE_TAC [LP_def, add_extend_l]);
-
-val L_LP = store_thm ("L_LP", ``extends L LP``,
-    REWRITE_TAC [LP_def, add_extend_r]);
-
 val _ = set_mapped_fixity { fixity = Infix(NONASSOC, 450), tok = "-->", term_name = "arrow" };
 val _ = Unicode.unicode_version {u = UnicodeChars.rightarrow, tmnm = "arrow"};
 
@@ -123,6 +97,28 @@ in
   and arrow_plus = store_thm ("arrow_plus", ``(!X A B. X A B ==> arrow A B)``, t)
 end;
 
+(** most popular extensions **)
+
+val NL_def = Define `NL = EMPTY_REL`;
+
+val (L_rules, _ , _) = Hol_reln `
+    (!A B C. L (Dot A (Dot B C)) (Dot (Dot A B) C)) /\
+    (!A B C. L (Dot (Dot A B) C) (Dot A (Dot B C))) `;
+
+val (NLP_rules, _, _) = Hol_reln `
+    (!A B. NLP (Dot A B) (Dot B A)) `;
+
+val LP_def = Define `LP = add_extension NLP L`;
+
+val NL_X = store_thm ("NL_X", ``!X. extends NL X``,
+    RW_TAC std_ss [extends_def, NL_def, EMPTY_REL_DEF, RSUBSET]);
+
+val NLP_LP = store_thm ("NLP_LP", ``extends NLP LP``,
+    REWRITE_TAC [LP_def, add_extend_l]);
+
+val L_LP = store_thm ("L_LP", ``extends L LP``,
+    REWRITE_TAC [LP_def, add_extend_r]);
+
 (* from p_arrow_rules to arrow_rules, this is actually all primitive rules for NL *)
 val arrow_rules = LIST_CONJ [one, comp, beta, beta', gamma, gamma', arrow_plus];
 
@@ -136,8 +132,8 @@ val Dot_mono_right = store_thm ("Dot_mono_right",
  >> MATCH_MP_TAC comp
  >> EXISTS_TAC ``B:'a Form``
  >> CONJ_TAC
- >| [ POP_ASSUM ACCEPT_TAC,
-      MATCH_MP_TAC gamma >> rw[one] ]);
+ >| [ ASM_REWRITE_TAC [],
+      MATCH_MP_TAC gamma >> RW_TAC std_ss [one] ]);
 
 val Dot_mono_left = store_thm ("Dot_mono_left",
   ``!A B A'. arrow A' A ==> arrow (Dot A' B) (Dot A B)``,
@@ -146,8 +142,8 @@ val Dot_mono_left = store_thm ("Dot_mono_left",
  >> MATCH_MP_TAC comp
  >> EXISTS_TAC ``A:'a Form``
  >> CONJ_TAC
- >| [ POP_ASSUM ACCEPT_TAC,
-      MATCH_MP_TAC beta >> rw[one] ]);
+ >| [ ASM_REWRITE_TAC [],
+      MATCH_MP_TAC beta >> RW_TAC std_ss [one] ]);
 		  
 val Dot_mono = store_thm ("Dot_mono",
   ``!A B C D. arrow A C /\ arrow B D ==> arrow (Dot A B) (Dot C D)``,
@@ -155,8 +151,8 @@ val Dot_mono = store_thm ("Dot_mono",
  >> MATCH_MP_TAC comp
  >> EXISTS_TAC ``Dot C B``
  >> CONJ_TAC
- >| [ MATCH_MP_TAC Dot_mono_left >> rw[],
-      MATCH_MP_TAC Dot_mono_right >> rw[] ]);
+ >| [ MATCH_MP_TAC Dot_mono_left >> RW_TAC std_ss [],
+      MATCH_MP_TAC Dot_mono_right >> RW_TAC std_ss [] ]);
 
 val Slash_mono_left = store_thm ("Slash_mono_left",
   ``!C B C'. arrow C' C ==> arrow (Slash C' B) (Slash C B)``,
@@ -165,7 +161,7 @@ val Slash_mono_left = store_thm ("Slash_mono_left",
  >> MATCH_MP_TAC comp
  >> EXISTS_TAC ``C':'a Form``
  >> CONJ_TAC
- >| [ MATCH_MP_TAC beta' >> rw[one], rw[] ]);
+ >| [ MATCH_MP_TAC beta' >> RW_TAC std_ss [one], RW_TAC std_ss [] ]);
 
 val Slash_antimono_right = store_thm ("Slash_antimono_right",
   ``!C B B'. arrow B' B ==> arrow (Slash C B) (Slash C B')``,
@@ -175,8 +171,8 @@ val Slash_antimono_right = store_thm ("Slash_antimono_right",
  >> MATCH_MP_TAC comp
  >> EXISTS_TAC ``B:'a Form``
  >> CONJ_TAC
- >| [ POP_ASSUM ACCEPT_TAC,
-      MATCH_MP_TAC gamma >> MATCH_MP_TAC beta' >> rw[one] ]);
+ >| [ ASM_REWRITE_TAC [],
+      MATCH_MP_TAC gamma >> MATCH_MP_TAC beta' >> RW_TAC std_ss [one] ]);
 
 val Backslash_antimono_left = store_thm ("Backslash_antimono_left",
   ``!A C A'. arrow A A' ==> arrow (Backslash A' C) (Backslash A C)``,
@@ -186,8 +182,8 @@ val Backslash_antimono_left = store_thm ("Backslash_antimono_left",
  >> MATCH_MP_TAC comp
  >> EXISTS_TAC ``A':'a Form``
  >> CONJ_TAC
- >| [ POP_ASSUM ACCEPT_TAC,
-      MATCH_MP_TAC beta >> MATCH_MP_TAC gamma' >> rw[one] ]);
+ >| [ ASM_REWRITE_TAC [],
+      MATCH_MP_TAC beta >> MATCH_MP_TAC gamma' >> RW_TAC std_ss [one] ]);
 
 val Backslash_mono_right = store_thm ("Backslash_mono_right",
   ``!A C C'. arrow C' C ==> arrow (Backslash A C') (Backslash A C)``,
@@ -196,17 +192,18 @@ val Backslash_mono_right = store_thm ("Backslash_mono_right",
  >> MATCH_MP_TAC comp
  >> EXISTS_TAC ``C':'a Form``
  >> CONJ_TAC
- >| [ MATCH_MP_TAC beta' >> MATCH_MP_TAC beta >> MATCH_MP_TAC gamma' >> rw[one],
-      POP_ASSUM ACCEPT_TAC ]);
+ >| [ MATCH_MP_TAC beta' >> MATCH_MP_TAC beta >>
+      MATCH_MP_TAC gamma' >> RW_TAC std_ss [one],
+      ASM_REWRITE_TAC [] ]);
 
 (* extended version of the arrow relation *)
 val Arrow_def = Define `Arrow X = add_extension arrow X`;
 
 val mono_X = store_thm ("mono_X",
-  ``!X X'. extends X X' ==> !A B. Arrow X A B ==> Arrow X' A B``,
+  ``!X X'. extends X X' ==> (!A B. Arrow X A B ==> Arrow X' A B)``,
     RW_TAC std_ss [extends_def, Arrow_def, add_extension_def, RSUBSET, RUNION]
-    THENL [ DISJ1_TAC >> rw[],
-	    DISJ2_TAC >> rw[] ]);
+    THENL [ DISJ1_TAC >> RW_TAC std_ss [],
+	    DISJ2_TAC >> RW_TAC std_ss [] ]);
 
 val X_Arrow = store_thm ("X_arrow", ``!X A B. X A B ==> Arrow X A B``,
     RW_TAC std_ss [Arrow_def, add_extension_def, RUNION, RSUBSET]);
@@ -305,30 +302,66 @@ val _ = add_rule { term_name = "Comma", fixity = Infix(LEFT, 500),
 
 val _ = type_abbrev ("gentzen_extension", ``:'a Term -> 'a Term -> bool``);
 
-val NL_Sequent_def = Define `NL_Sequent = EMPTY_REL`;
+(* Definition of the recursive function that translates Terms to Forms *)
+val deltaTranslation_def = Define `
+    (deltaTranslation (OneForm f) = f) /\
+    (deltaTranslation (Comma t1 t2) = Dot (deltaTranslation t1) (deltaTranslation t2))`;
 
-val (NLP_Sequent_rules, _ , _) = Hol_reln `
-    (!A B. NLP_Sequent (Comma A B) (Comma B A))`; (* NLP_Intro *)
+(* Definition of the relation that connects arrow_extension with gentzen_extension *)
+val implements_def = Define
+   `implements (X:'a arrow_extension) (E:'a gentzen_extension) =
+    (!(A:'a Term) (B:'a Term). E A B = X (deltaTranslation A) (deltaTranslation B))`;
 
-val (L_Sequent_rules, _ , _) = Hol_reln `
-    (!A B C. L_Sequent (Comma A (Comma B C)) (Comma (Comma A B) C)) /\	(* L_Intro_lr *)
-    (!A B C. L_Sequent (Comma (Comma A B) C) (Comma A (Comma B C))) `;	(* L_Intro_rl *)
+(* NL Sequent extension, an empty relation actually *)
+val NL_Sequent_def = Define `NL_Sequent A B = NL (deltaTranslation A) (deltaTranslation B)`;
+
+val NL_implements_NL_Sequent = store_thm ("NL_implements_NL_Sequent",
+  ``implements NL NL_Sequent``,
+    RW_TAC std_ss [NL_Sequent_def, implements_def]);
+
+(* NLP Sequent extension *)
+val NLP_Sequent_def = Define `NLP_Sequent A B = NLP (deltaTranslation A) (deltaTranslation B)`;
+
+val NLP_implements_NLP_Sequent = store_thm ("NLP_implements_NLP_Sequent",
+  ``implements NLP NLP_Sequent``,
+    RW_TAC std_ss [NLP_Sequent_def, implements_def]);
+
+val NLP_Intro = store_thm ("NLP_Intro", ``!A B. NLP_Sequent (Comma A B) (Comma B A)``,
+    RW_TAC std_ss [deltaTranslation_def, NLP_Sequent_def, NLP_rules]);
+
+(* L Sequent extension, the Full Lambek Sequent Calculus extension *)
+val L_Sequent_def = Define `L_Sequent A B = L (deltaTranslation A) (deltaTranslation B)`;
+
+val L_implements_L_Sequent = store_thm ("L_implements_L_Sequent",
+  ``implements L L_Sequent``,
+    RW_TAC std_ss [L_Sequent_def, implements_def]);
+
+(* two important L_Intro rules now become theorems *)
+local
+  val t = RW_TAC std_ss [deltaTranslation_def, L_Sequent_def, L_rules]
+in
+  val L_Intro_lr = store_thm ("L_Intro_lr",
+    ``!A B C. L_Sequent (Comma A (Comma B C)) (Comma (Comma A B) C)``, t)
+  and L_Intro_rl = store_thm ("L_Intro_rl",
+    ``!A B C. L_Sequent (Comma (Comma A B) C) (Comma A (Comma B C))``, t)
+end;
 
 val LP_Sequent_def = Define `LP_Sequent = add_extension NLP_Sequent L_Sequent`;
 
 val LP_extends_L = store_thm ("LP_extends_L",
-    ``!E. extends LP_Sequent E ==> extends L_Sequent E``,
+  ``!E. extends LP_Sequent E ==> extends L_Sequent E``,
     RW_TAC std_ss [LP_Sequent_def, extends_def, add_extension_def, RSUBSET, RUNION]);
 
 val LP_extends_NLP = store_thm ("LP_extends_NLP",
-    ``!E. extends LP_Sequent E ==> extends NLP_Sequent E``,
+  ``!E. extends LP_Sequent E ==> extends NLP_Sequent E``,
     RW_TAC std_ss [LP_Sequent_def, extends_def, add_extension_def, RSUBSET, RUNION]);
 
-(* Definition of the function that translates Terms to Forms *)
-val deltaTranslation_def = Define `
-    ((deltaTranslation:'a Term->'a Form) (OneForm f) = f) /\
-    ((deltaTranslation:'a Term->'a Form) (Comma t1 t2) =
-	Dot (deltaTranslation t1) (deltaTranslation t2))`;
+val LP_implements_LP_Sequent = store_thm ("LP_implements_LP_Sequent",
+  ``implements LP LP_Sequent``,
+    REWRITE_TAC [implements_def]
+ >> RW_TAC std_ss [LP_def, LP_Sequent_def]
+ >> REWRITE_TAC [add_extension_def, RUNION]
+ >> RW_TAC std_ss [NLP_Sequent_def, L_Sequent_def]);
 
 (*** Module: ReplaceProp ***)
 
@@ -393,13 +426,6 @@ in
   val replaceCommaDot_rules = LIST_CONJ [noReplace, replaceOneComma, replaceOneComma']
 end;
 
-(* original definition, for reference purposes only
-val (replaceCommaDotX_rules, replaceCommaDotX_ind, replaceCommaDotX_cases) = Hol_reln `
-    (!T1. replaceCommaDotX T1 T1) /\
-    (!T1 T2 T3 A B. replace T1 T2 (Comma (OneForm A) (OneForm B)) (OneForm (Dot A B)) /\
-		    replaceCommaDotX T2 T3 ==> replaceCommaDotX T1 T3)`;
- *)
-
 (* An induction theorem for RTC replaceCommaDot1, similar to those generated by Hol_reln *)
 val replaceCommaDot_ind = store_thm ("replaceCommaDot_ind",
   ``!(P:'a gentzen_extension).
@@ -433,41 +459,418 @@ val replaceMono = store_thm ("replaceMono",
  >> EXISTS_TAC ``Comma T2 T3``
  >> PROVE_TAC [replaceMonoLeft, replaceMonoRight]);
 
-(* TODO
 val replaceTranslation = store_thm ("replaceTranslation",
   ``!T. replaceCommaDot T (OneForm (deltaTranslation T))``,
- *)
+    Induct
+ >| [ PROVE_TAC [deltaTranslation_def, noReplace], (* base case *)
+      REWRITE_TAC [deltaTranslation_def]         (* induct case *)
+   >> MATCH_MP_TAC replaceTransitive'
+   >> EXISTS_TAC ``Comma (OneForm (deltaTranslation T')) (OneForm (deltaTranslation T''))``
+   >> PROVE_TAC [replaceOneComma, noReplace, replaceRoot, replaceMono] ]);
+
+(* TODO / remain theorems: replace_inv1, replace_inv2, doubleReplace, replaceSameP, replaceTrans *)
 
 (*** Module: NaturalDeduction ***)
 
-val _ = set_mapped_fixity { fixity = Infix(NONASSOC, 450), tok = "|-", term_name = "natDed" };
+(* TODO: possible alternative definition, the rest rules then become theorems
+val natDed'_def = Define `
+    natDed' E Gamma A = (!X. implements X E /\ Arrow X (deltaTranslation Gamma) A)`;
+ *)
 
-(* TODO: can Natural Deduction rules be derived from arrow rules and deltaTranslation ? *)
-val (natDed_rules, _ , _ ) = Hol_reln `
-    (!A. natDed (OneForm A) A) /\						(* NatAxiom *)
-    (!Gamma A B. natDed (Comma Gamma (OneForm B)) A				(* SlashIntro *)
-		 ==>	
-		 natDed Gamma (Slash A B)) /\
-    (!Gamma A B. natDed (Comma (OneForm B) Gamma) A				(* BackslashIntro *)
-		 ==>
-		 natDed Gamma (Backslash B A)) /\
-    (!Gamma Delta A B. (natDed Gamma A /\ natDed Delta B)			(* DotIntro *)
-		       ==>
-		       natDed (Comma Gamma Delta) (Dot A B)) /\
-    (!Gamma Delta A B. (natDed Gamma (Slash A B) /\ natDed Delta B) ==>		(* SlashElim *)
-		       natDed (Comma Gamma Delta) A) /\
-    (!Gamma Delta A B. (natDed Gamma B /\ natDed Delta (Backslash B A)) ==>	(* BackslashElim *)
-		       natDed (Comma Gamma Delta) A) /\
-    (!Gamma Gamma' Delta A B C.							(* DotElim *)
-     (replace Gamma Gamma' (Comma (OneForm A) (OneForm B)) Delta
-      /\ natDed Delta (Dot A B) /\ natDed Gamma C) ==> natDed Gamma' C) /\
-    (!N:'a gentzen_extension Gamma Gamma' T1 T2 C.				(* NatExt *)
-     (N T1 T2 /\ replace Gamma Gamma' T1 T2 /\ natDed Gamma C) ==> natDed Gamma' C) `;
+val (natDed_rules, _ , _) = Hol_reln `
+    (!A (E:'a gentzen_extension). natDed E (OneForm A) A) /\			(* NatAxiom *)
+    (!Gamma A B E.								(* SlashIntro *)
+      natDed E (Comma Gamma (OneForm B)) A ==> natDed E Gamma (Slash A B)) /\
+    (!Gamma A B E.								(* BackslashIntro *)
+      natDed E (Comma (OneForm B) Gamma) A ==> natDed E Gamma (Backslash B A)) /\
+    (!Gamma Delta A B E.							(* DotIntro *)
+      natDed E Gamma A /\ natDed E Delta B ==> natDed E (Comma Gamma Delta) (Dot A B)) /\
+    (!Gamma Delta A B E.							(* SlashElim *)
+      natDed E Gamma (Slash A B) /\ natDed E Delta B ==> natDed E (Comma Gamma Delta) A) /\
+    (!Gamma Delta A B E.						 	(* BackslashElim *)
+      natDed E Gamma B /\ natDed E Delta (Backslash B A) ==> natDed E (Comma Gamma Delta) A) /\
+    (!Gamma Gamma' Delta A B C E.						(* DotElim *)
+      replace Gamma Gamma' (Comma (OneForm A) (OneForm B)) Delta /\
+      natDed E Delta (Dot A B) /\ natDed E Gamma C ==> natDed E Gamma' C) /\
+    (!(N:'a gentzen_extension) Gamma Gamma' T1 T2 C E.				(* NatExt *)
+      N T1 T2 /\ replace Gamma Gamma' T1 T2 /\ natDed E Gamma C ==> natDed E Gamma' C)`;
 
 (* Break above rules into separated theorems with proper names *)
 val [NatAxiom, SlashIntro, BackslashIntro, DotIntro, SlashElim, BackslashElim, DotElim, NatExt] =
-    CONJ_LIST 8 natDed_rules;
+    (CONJ_LIST 8 natDed_rules);
+
+val NatAxiomGen = store_thm ("NatAxiomGen", ``!Gamma E. natDed E Gamma (deltaTranslation Gamma)``,
+    Induct
+ >| [ PROVE_TAC [deltaTranslation_def, NatAxiom], (* base case *)
+      REWRITE_TAC [deltaTranslation_def] >>     (* induct case *)
+      PROVE_TAC [DotIntro] ]);
+
+val DotElimGeneralized = store_thm ("DotElimGeneralized",
+  ``!E T1 T2 C. replaceCommaDot T1 T2 /\ natDed E T1 C ==> natDed E T2 C``,
+    PROVE_TAC [replace_rules, replaceCommaDot_rules, natDed_rules]);
+
+(*** Module: Sequent Calculus ***)
+
+(* TODO: possible alternative definition, the rest rules then become theorems
+val (gentzenSequent'_rules, _ , _) = Hol_reln `
+    (!Gamma A X E.
+      implements X E /\ Arrow X (deltaTranslation Gamma) A
+      ==> gentzenSequent' E Gamma A) /\
+    (!Delta Gamma Gamma' A C E.							(* CutRule *)
+      replace Gamma Gamma' (OneForm A) Delta /\
+      gentzenSequent' E Delta A /\ gentzenSequent' E Gamma C
+      ==> gentzenSequent' E Gamma' C)`;
+ *)
+
+val (gentzenSequent_rules, _ , _) = Hol_reln `
+    (!A (E:'a gentzen_extension). gentzenSequent E (OneForm A) A) /\		(* SeqAxiom *)
+    (!Gamma A B E.								(* RightSlash *)
+      gentzenSequent E (Comma Gamma (OneForm B)) A ==>
+      gentzenSequent E Gamma (Slash A B)) /\
+    (!Gamma A B E.								(* RightBackslash *)
+      gentzenSequent E (Comma (OneForm B) Gamma) A ==>
+      gentzenSequent E Gamma (Backslash B A)) /\
+    (!Gamma Delta A B E.							(* RightDot *)
+      gentzenSequent E Gamma A /\ gentzenSequent E Delta B
+      ==> gentzenSequent E (Comma Gamma Delta) (Dot A B)) /\
+    (!Gamma Gamma' Delta A B C E.						(* LeftSlash *)
+      replace Gamma Gamma' (OneForm A) (Comma (OneForm (Slash A B)) Delta) /\
+      gentzenSequent E Delta B /\ gentzenSequent E Gamma C
+      ==> gentzenSequent E Gamma' C) /\
+    (!Gamma Gamma' Delta A B C E.						(* LeftBackslash *)
+      replace Gamma Gamma' (OneForm A) (Comma Delta (OneForm (Backslash B A))) /\
+      gentzenSequent E Delta B /\ gentzenSequent E Gamma C
+      ==> gentzenSequent E Gamma' C) /\
+    (!Gamma Gamma' A B C E.							(* LeftDot *)
+      replace Gamma Gamma' (Comma (OneForm A) (OneForm B)) (OneForm (Dot A B)) /\
+      gentzenSequent E Gamma C
+      ==> gentzenSequent E Gamma' C) /\
+    (!Delta Gamma Gamma' A C E.							(* CutRule *)
+      replace Gamma Gamma' (OneForm A) Delta /\
+      gentzenSequent E Delta A /\ gentzenSequent E Gamma C
+      ==> gentzenSequent E Gamma' C) /\
+    (!(N:'a gentzen_extension) Gamma Gamma' T1 T2 C E.				(* SequentExtension *)
+      N T1 T2 /\ replace Gamma Gamma' T1 T2 /\ gentzenSequent E Gamma C
+      ==> gentzenSequent E Gamma' C)`;
+
+val [SeqAxiom, RightSlash, RightBackslash, RightDot, LeftSlash, LeftBackslash, LeftDot,
+     CutRule, SequentExtension] =
+    (CONJ_LIST 9 gentzenSequent_rules);
+
+val SeqAxiomGen = store_thm ("SeqAxiomGen", ``!Gamma E. gentzenSequent E Gamma (deltaTranslation Gamma)``,
+    Induct
+ >| [ PROVE_TAC [deltaTranslation_def, SeqAxiom], (* base case *)
+      REWRITE_TAC [deltaTranslation_def] >>     (* induct case *)
+      PROVE_TAC [RightDot] ]);
+
+(* Some derived properties concerning gentzenSequent *)
+
+val LeftDotSimpl = store_thm ("LeftDotSimpl",
+  ``!A B C E. gentzenSequent E (Comma (OneForm A) (OneForm B)) C ==>
+	      gentzenSequent E (OneForm (Dot A B)) C``,
+    REPEAT STRIP_TAC
+ >> MATCH_MP_TAC LeftDot
+ >> EXISTS_TAC ``(Comma (OneForm A) (OneForm B))``
+ >> EXISTS_TAC ``A:'a Form``
+ >> EXISTS_TAC ``B:'a Form``
+ >> PROVE_TAC [replaceRoot]);
+
+val LeftDotGeneralized = store_thm ("LeftDotGeneralized",
+  ``!T1 T2 C E. replaceCommaDot T1 T2 /\ gentzenSequent E T1 C ==> gentzenSequent E T2 C``,
+    PROVE_TAC [replace_rules, replaceCommaDot_rules, gentzenSequent_rules]);
+
+val TermToForm = store_thm ("TermToForm",
+  ``!Gamma C E. gentzenSequent E Gamma C
+	    ==> gentzenSequent E (OneForm (deltaTranslation Gamma)) C``,
+    REPEAT STRIP_TAC
+ >> MATCH_MP_TAC LeftDotGeneralized
+ >> EXISTS_TAC ``Gamma:'a Term``
+ >> RW_TAC std_ss [replaceTranslation]);
+
+val LeftSlashSimpl = store_thm ("LeftSlashSimpl",
+  ``!Gamma A B C E. gentzenSequent E Gamma B /\ gentzenSequent E (OneForm A) C
+	        ==> gentzenSequent E (Comma (OneForm (Slash A B)) Gamma) C``,
+    PROVE_TAC [replace_rules, replaceCommaDot_rules, LeftSlash]);
+
+val LeftBackslashSimpl = store_thm ("LeftBackslashSimpl",
+  ``!Gamma A B C E. gentzenSequent E Gamma B /\ gentzenSequent E (OneForm A) C
+	        ==> gentzenSequent E (Comma Gamma (OneForm (Backslash B A))) C``,
+    PROVE_TAC [replace_rules, replaceCommaDot_rules, LeftBackslash]);
+
+val CutRuleSimpl = store_thm ("CutRuleSimpl",
+  ``!Gamma A C E. gentzenSequent E Gamma A /\ gentzenSequent E (OneForm A) C
+	      ==> gentzenSequent E Gamma C``,
+    PROVE_TAC [replace_rules, replaceCommaDot_rules, CutRule]);
+
+val DotRightSlash' = store_thm ("DotRightSlash'",
+  ``!A B C E. gentzenSequent E (OneForm A) (Slash C B)
+	  ==> gentzenSequent E (OneForm (Dot A B)) C``,
+    PROVE_TAC [replace_rules, replaceCommaDot_rules, gentzenSequent_rules]);
+
+val DotRightBackslash' = store_thm ("DotRightBackslash'",
+  ``!A B C E. gentzenSequent E (OneForm B) (Backslash A C)
+	  ==> gentzenSequent E (OneForm (Dot A B)) C``,
+    PROVE_TAC [replace_rules, replaceCommaDot_rules, gentzenSequent_rules]);
+
+(* some definitions concerning extensions *)
+
+val LextensionSimpl = store_thm ("LextensionSimpl",
+  ``!T1 T2 T3 C E. extends L_Sequent E /\
+		   gentzenSequent E (Comma T1 (Comma T2 T3)) C
+	       ==> gentzenSequent E (Comma (Comma T1 T2) T3) C``,
+    REPEAT STRIP_TAC
+ >> MATCH_MP_TAC SequentExtension
+ >> EXISTS_TAC ``L_Sequent:'a gentzen_extension`` (* E *)
+ >> EXISTS_TAC ``(Comma T1 (Comma T2 T3))``       (* Gamma *)
+ >> EXISTS_TAC ``(Comma T1 (Comma T2 T3))``       (* T1 *)
+ >> EXISTS_TAC ``(Comma (Comma T1 T2) T3)``       (* T2 *)
+ >> RW_TAC std_ss [extends_def, RUNION, replaceRoot, L_Intro_lr]);
+
+val LextensionSimpl' = store_thm ("LextensionSimpl'", (* dual theorem of above *)
+  ``!T1 T2 T3 C E. extends L_Sequent E /\
+		   gentzenSequent E (Comma (Comma T1 T2) T3) C
+	       ==> gentzenSequent E (Comma T1 (Comma T2 T3)) C``,
+    REPEAT STRIP_TAC
+ >> MATCH_MP_TAC SequentExtension
+ >> EXISTS_TAC ``L_Sequent:'a gentzen_extension`` (* E *)
+ >> EXISTS_TAC ``(Comma (Comma T1 T2) T3)``       (* Gamma *)
+ >> EXISTS_TAC ``(Comma (Comma T1 T2) T3)``       (* T1 *)
+ >> EXISTS_TAC ``(Comma T1 (Comma T2 T3))``       (* T2 *)
+ >> RW_TAC std_ss [extends_def, RUNION, replaceRoot, L_Intro_rl]);
+
+val LextensionSimplDot = store_thm ("LextensionSimplDot",
+  ``!A B C D E. extends L_Sequent E /\
+		gentzenSequent E (OneForm (Dot A (Dot B C))) D
+	    ==> gentzenSequent E (OneForm (Dot (Dot A B) C)) D``,
+    REPEAT STRIP_TAC
+ >> MATCH_MP_TAC LeftDotSimpl
+ >> MATCH_MP_TAC LeftDot
+ >> EXISTS_TAC ``(Comma (Comma (OneForm A) (OneForm B)) (OneForm C))``
+ >> EXISTS_TAC ``A:'a Form``
+ >> EXISTS_TAC ``B:'a Form``
+ >> STRIP_TAC
+ >| [ RW_TAC std_ss [replaceLeft, replaceRoot],
+      MATCH_MP_TAC LextensionSimpl
+   >> STRIP_TAC
+   >| [ ASM_REWRITE_TAC [],
+	MATCH_MP_TAC CutRuleSimpl
+     >> EXISTS_TAC ``(deltaTranslation (Comma (OneForm A) (Comma (OneForm B) (OneForm C))))``
+     >> RW_TAC std_ss [SeqAxiomGen, deltaTranslation_def] ] ]);
+
+val LextensionSimplDot' = store_thm ("LextensionSimplDot'", (* dual theorem of above *)
+  ``!A B C D E. extends L_Sequent E /\
+		gentzenSequent E (OneForm (Dot (Dot A B) C)) D
+	    ==> gentzenSequent E (OneForm (Dot A (Dot B C))) D``,
+    REPEAT STRIP_TAC
+ >> MATCH_MP_TAC LeftDotSimpl
+ >> MATCH_MP_TAC LeftDot
+ >> EXISTS_TAC ``(Comma (OneForm A) (Comma (OneForm B) (OneForm C)))``
+ >> EXISTS_TAC ``B:'a Form``
+ >> EXISTS_TAC ``C:'a Form``
+ >> STRIP_TAC
+ >| [ RW_TAC std_ss [replaceRight, replaceRoot],
+      MATCH_MP_TAC LextensionSimpl'
+   >> STRIP_TAC
+   >| [ ASM_REWRITE_TAC [],
+	MATCH_MP_TAC CutRuleSimpl
+     >> EXISTS_TAC ``(deltaTranslation (Comma (Comma (OneForm A) (OneForm B)) (OneForm C)))``
+     >> RW_TAC std_ss [SeqAxiomGen, deltaTranslation_def] ] ]);
+
+val NLPextensionSimpl = store_thm ("NLPextensionSimpl",
+  ``!T1 T2 C E. extends NLP_Sequent E /\
+		gentzenSequent E (Comma T1 T2) C
+	    ==> gentzenSequent E (Comma T2 T1) C``,
+    REPEAT STRIP_TAC
+ >> MATCH_MP_TAC SequentExtension
+ >> EXISTS_TAC ``NLP_Sequent:'a gentzen_extension``
+ >> EXISTS_TAC ``(Comma T1 T2)``
+ >> EXISTS_TAC ``(Comma T1 T2)``
+ >> EXISTS_TAC ``(Comma T2 T1)``
+ >> RW_TAC std_ss [extends_def, RUNION, replaceRoot, NLP_Intro]);
+
+val NLPextensionSimplDot = store_thm ("NLPextensionSimplDot",
+  ``!A B C E. extends NLP_Sequent E /\
+	      gentzenSequent E (OneForm (Dot A B)) C
+	  ==> gentzenSequent E (OneForm (Dot B A)) C``,
+    REPEAT STRIP_TAC
+ >> MATCH_MP_TAC LeftDotSimpl
+ >> MATCH_MP_TAC NLPextensionSimpl
+ >> STRIP_TAC
+ >| [ ASM_REWRITE_TAC [],
+      MATCH_MP_TAC CutRuleSimpl
+   >> EXISTS_TAC ``(deltaTranslation (Comma (OneForm A) (OneForm B)))``
+   >> RW_TAC std_ss [SeqAxiomGen, deltaTranslation_def] ]);
+
+(* not needed for now
+val mono_E = store_thm ("mono_E", (* original name: gentzenExtends, see also mono_X *)
+  ``!E E'. extends E E' ==> (!Gamma A. gentzenSequent E Gamma A ==> gentzenSequent E' Gamma A)``,
+    RW_TAC std_ss [extends_def, RSUBSET]
+ >> PROVE_TAC [gentzenSequent_rules]
+ >> );
+ *)
+
+(* Some theorems and derived properties
+   These definitions can be applied for all gentzen extensions,
+   we can see how CutRuleSimpl gets used in most of time. *)
+
+val application = store_thm ("application",
+  ``!A B E. gentzenSequent E (OneForm (Dot (Slash A B) B)) A``,
+    PROVE_TAC [LeftDotSimpl, LeftSlashSimpl, SeqAxiom]);
+
+val application' = store_thm ("application'",
+  ``!A B E. gentzenSequent E (OneForm (Dot B (Backslash B A))) A``,
+    PROVE_TAC [LeftDotSimpl, LeftBackslashSimpl, SeqAxiom]);
+
+val RightSlashDot = store_thm ("RightSlashDot",
+  ``!A B C E. gentzenSequent E (OneForm (Dot A C)) B ==> gentzenSequent E (OneForm A) (Slash B C)``,
+    REPEAT STRIP_TAC
+ >> MATCH_MP_TAC RightSlash
+ >> MATCH_MP_TAC CutRuleSimpl
+ >> EXISTS_TAC ``(deltaTranslation (Comma (OneForm A) (OneForm C)))``
+ >> RW_TAC std_ss [SeqAxiomGen, deltaTranslation_def]);
+
+val coApplication = store_thm ("coApplication",
+  ``!A B E. gentzenSequent E (OneForm A) (Slash (Dot A B) B)``,
+    PROVE_TAC [RightSlash, RightDot, SeqAxiom]);
+
+val coApplication' = store_thm ("coApplication'",
+  ``!A B E. gentzenSequent E (OneForm A) (Backslash B (Dot B A))``,
+    PROVE_TAC [RightBackslash, RightDot, SeqAxiom]);
+
+val monotonicity = store_thm ("monotonicity",
+  ``!A B C D E. gentzenSequent E (OneForm A) B /\
+		gentzenSequent E (OneForm C) D
+	    ==> gentzenSequent E (OneForm (Dot A C)) (Dot B D)``,
+    PROVE_TAC [LeftDotSimpl, RightDot]);
+
+val isotonicity = store_thm ("isotonicity",
+  ``!A B C E. gentzenSequent E (OneForm A) B
+	  ==> gentzenSequent E (OneForm (Slash A C)) (Slash B C)``,
+    REPEAT STRIP_TAC
+ >> MATCH_MP_TAC RightSlash
+ >> MATCH_MP_TAC CutRuleSimpl
+ >> EXISTS_TAC ``A:'a Form``
+ >> PROVE_TAC [LeftSlashSimpl, SeqAxiom]);
+
+val isotonicity' = store_thm ("isotonicity'",
+  ``!A B C E. gentzenSequent E (OneForm A) B
+	  ==> gentzenSequent E (OneForm (Backslash C A)) (Backslash C B)``,
+    REPEAT STRIP_TAC
+ >> MATCH_MP_TAC RightBackslash
+ >> MATCH_MP_TAC CutRuleSimpl
+ >> EXISTS_TAC ``A:'a Form``
+ >> PROVE_TAC [LeftBackslashSimpl, SeqAxiom]);
+
+val antitonicity = store_thm ("antitonicity",
+  ``!A B C E. gentzenSequent E (OneForm A) B
+	  ==> gentzenSequent E (OneForm (Slash C B)) (Slash C A)``,
+    REPEAT STRIP_TAC
+ >> MATCH_MP_TAC RightSlash
+ >> MATCH_MP_TAC CutRuleSimpl
+ >> EXISTS_TAC ``(Dot (Slash C B) B)``
+ >> STRIP_TAC
+ >| [ PROVE_TAC [RightDot, SeqAxiom],
+      REWRITE_TAC [application] ]);
+
+val antitonicity' = store_thm ("antitonicity'",
+  ``!A B C E. gentzenSequent E (OneForm A) B
+	  ==> gentzenSequent E (OneForm (Backslash B C)) (Backslash A C)``,
+    REPEAT STRIP_TAC
+ >> MATCH_MP_TAC RightBackslash
+ >> MATCH_MP_TAC CutRuleSimpl
+ >> EXISTS_TAC ``(Dot B (Backslash B C))``
+ >> STRIP_TAC
+ >| [ PROVE_TAC [RightDot, SeqAxiom],
+      REWRITE_TAC [application'] ]);
+
+val lifting = store_thm ("lifting",
+  ``!A B C E. gentzenSequent E (OneForm A) (Slash B (Backslash A B))``,
+    REPEAT STRIP_TAC
+ >> MATCH_MP_TAC RightSlash
+ >> MATCH_MP_TAC CutRuleSimpl
+ >> EXISTS_TAC ``(Dot A (Backslash A B))``
+ >> STRIP_TAC
+ >| [ PROVE_TAC [RightDot, SeqAxiom],
+      REWRITE_TAC [application'] ]);
+
+val lifting' = store_thm ("lifting'",
+  ``!A B C E. gentzenSequent E (OneForm A) (Backslash (Slash B A) B)``,
+    REPEAT STRIP_TAC
+ >> MATCH_MP_TAC RightBackslash
+ >> MATCH_MP_TAC CutRuleSimpl
+ >> EXISTS_TAC ``(Dot (Slash B A) A)``
+ >> STRIP_TAC
+ >| [ PROVE_TAC [RightDot, SeqAxiom],
+      REWRITE_TAC [application] ]);
+
+(* These definitions can be applied iff associativity is supported by our logical system *)
+
+val mainGeach = store_thm ("mainGeach",
+  ``!A B C E. extends L_Sequent E ==>
+       gentzenSequent E (OneForm (Slash A B)) (Slash (Slash A C) (Slash B C))``,
+    REPEAT STRIP_TAC
+ >> NTAC 2 (MATCH_MP_TAC RightSlash)
+ >> MATCH_MP_TAC LextensionSimpl
+ >> STRIP_TAC THEN1 (POP_ASSUM ACCEPT_TAC)
+ >> MATCH_MP_TAC CutRuleSimpl
+ >> EXISTS_TAC ``(Dot (Slash A B) B)``
+ >> STRIP_TAC
+ >| [ MATCH_MP_TAC RightDot >> STRIP_TAC >|
+      [ REWRITE_TAC [SeqAxiom],
+        MATCH_MP_TAC LeftSlashSimpl >> STRIP_TAC >> REWRITE_TAC [SeqAxiom] ] ,
+      REWRITE_TAC [application] ]);
+
+val mainGeach' = store_thm ("mainGeach'",
+  ``!A B C E. extends L_Sequent E ==>
+       gentzenSequent E (OneForm (Backslash B A)) (Backslash (Backslash C B) (Backslash C A))``,
+    REPEAT STRIP_TAC
+ >> NTAC 2 (MATCH_MP_TAC RightBackslash)
+ >> MATCH_MP_TAC LextensionSimpl'
+ >> STRIP_TAC THEN1 (POP_ASSUM ACCEPT_TAC)
+ >> MATCH_MP_TAC CutRuleSimpl
+ >> EXISTS_TAC ``(Dot B (Backslash B A))``
+ >> STRIP_TAC
+ >| [ MATCH_MP_TAC RightDot >> STRIP_TAC >|
+      [ MATCH_MP_TAC LeftBackslashSimpl >> STRIP_TAC >> REWRITE_TAC [SeqAxiom],
+	REWRITE_TAC [SeqAxiom] ] ,
+      REWRITE_TAC [application'] ]);
+
+val secondaryGeach = store_thm ("secondaryGeach",
+  ``!A B C E. extends L_Sequent E ==>
+       gentzenSequent E (OneForm (Slash B C)) (Backslash (Slash A B) (Slash A C))``,
+    REPEAT STRIP_TAC
+ >> MATCH_MP_TAC RightBackslash
+ >> MATCH_MP_TAC RightSlash
+ >> MATCH_MP_TAC LextensionSimpl
+ >> STRIP_TAC THEN1 (POP_ASSUM ACCEPT_TAC)
+ >> MATCH_MP_TAC CutRuleSimpl
+ >> EXISTS_TAC ``(Dot (Slash A B) B)``
+ >> STRIP_TAC
+ >| [ MATCH_MP_TAC RightDot >> STRIP_TAC >|
+      [ REWRITE_TAC [SeqAxiom],
+	MATCH_MP_TAC LeftSlashSimpl >> STRIP_TAC >> REWRITE_TAC [SeqAxiom] ] ,
+      REWRITE_TAC [application] ]);
+
+val secondaryGeach' = store_thm ("secondaryGeach'",
+  ``!A B C E. extends L_Sequent E ==>
+       gentzenSequent E (OneForm (Backslash C B)) (Slash (Backslash C A) (Backslash B A))``,
+    REPEAT STRIP_TAC
+ >> MATCH_MP_TAC RightSlash
+ >> MATCH_MP_TAC RightBackslash
+ >> MATCH_MP_TAC LextensionSimpl'
+ >> STRIP_TAC THEN1 (POP_ASSUM ACCEPT_TAC)
+ >> MATCH_MP_TAC CutRuleSimpl
+ >> EXISTS_TAC ``(Dot B (Backslash B A))``
+ >> STRIP_TAC
+ >| [ MATCH_MP_TAC RightDot >> STRIP_TAC >|
+      [ MATCH_MP_TAC LeftBackslashSimpl >> STRIP_TAC >> REWRITE_TAC [SeqAxiom],
+	REWRITE_TAC [SeqAxiom] ] ,
+      REWRITE_TAC [application'] ]);
 
 
 
+
+  
 val _ = export_theory ();
+
+(* last updated: January 8, 2016 *)
